added documentation, almost passing elaborator

Dex001/Dex001.fst
@@ -25,8 +25,8 @@ type d64 = { hi:U64.t; lo:U64.t }
 
 // multiply two uint64s without overflow
 // algorithm adapted from 'The Art of Computer Programming' by Donald E. Knuth
-val dmul64: U64.t -> U64.t -> d64 `cost` 0
-let dmul64 x y = let open U64 in
+val dmul64: U64.t -> U64.t -> d64 `cost` 39
+let dmul64 x y = let open U64 in // 39
     let m32 = 4294967296UL in // 2^32
     let xhi = x %^ m32 in // 32 high bits of x
     let xlo = x /^ m32 in // 32 low bits of x
@@ -41,32 +41,32 @@ let dmul64 x y = let open U64 in
     let lo = ((t2 *%^ m32) *%^ m32) +%^ (t0 %^ m32) in
     ret ({hi=hi; lo=lo})
 
-val mkAsset: contractId -> hash -> asset `cost` 0
-let mkAsset (version, contractHash) hash =
+val mkAsset: contractId -> hash -> asset `cost` 4
+let mkAsset (version, contractHash) hash = // 4
     ret (version, contractHash, hash)
 
-val hashAsset: asset -> hash `cost` 404
-let hashAsset asset =
+val hashAsset: asset -> hash `cost` 408
+let hashAsset asset = // 4
     Hash.updateAsset asset Hash.empty // 384
     >>= Hash.finalize // 20
 
-val hashU64: U64.t -> hash `cost` 68
-let hashU64 x =
+val hashU64: U64.t -> hash `cost` 72
+let hashU64 x = // 4
     Hash.updateU64 x Hash.empty // 48
     >>= Hash.finalize // 20
 
-val hashPubkey: publicKey -> hash `cost` 404
-let hashPubkey pk =
+val hashPubkey: publicKey -> hash `cost` 408
+let hashPubkey pk = // 4
     Hash.updateByteArray pk Hash.empty // 384
     >>= Hash.finalize // 20
 
-val hashOrder: order -> hash `cost` 2328
-let hashOrder order =
-    let! underlyingAssetHash = hashAsset order.underlyingAsset in // 404
-    let! underlyingAmountHash = hashU64 order.underlyingAmount in // 68
-    let! pairAssetHash = hashAsset order.pairAsset in // 404
-    let! orderTotalHash = hashU64 order.orderTotal in // 68
-    let! makerPubKeyHash = hashPubkey order.makerPubKey in // 404
+val hashOrder: order -> hash `cost` 2384
+let hashOrder order = // 36
+    let! underlyingAssetHash = hashAsset order.underlyingAsset in // 408
+    let! underlyingAmountHash = hashU64 order.underlyingAmount in // 72
+    let! pairAssetHash = hashAsset order.pairAsset in // 408
+    let! orderTotalHash = hashU64 order.orderTotal in // 72
+    let! makerPubKeyHash = hashPubkey order.makerPubKey in // 408
         Hash.updateHash underlyingAssetHash Hash.empty // 192
     >>= Hash.updateHash underlyingAmountHash // 192
     >>= Hash.updateHash pairAssetHash // 192
@@ -74,8 +74,8 @@ let hashOrder order =
     >>= Hash.updateHash makerPubKeyHash // 192
     >>= Hash.finalize // 20
 
-val getUnderlyingAsset: option (Dict.t data) -> result asset `cost` 198
-let getUnderlyingAsset dict =
+val getUnderlyingAsset: option (Dict.t data) -> result asset `cost` 241
+let getUnderlyingAsset dict = // 43
     let! version = dict >!= Dict.tryFind "UnderlyingAssetVersion" // 64
                         >?= tryU32 in // 2
     let! contractHash = dict >!= Dict.tryFind "UnderlyingContractHash" // 64
@@ -92,8 +92,8 @@ let getUnderlyingAsset dict =
     | _, _, None ->
         RT.failw "Message Body must include valid UnderlyingSubIdentifier"
 
-val getUnderlyingAmount: option (Dict.t data) -> result U64.t `cost` 66
-let getUnderlyingAmount dict =
+val getUnderlyingAmount: option (Dict.t data) -> result U64.t `cost` 79
+let getUnderlyingAmount dict = // 13
     let! underlyingAmount = dict >!= Dict.tryFind "UnderlyingAmount" // 64
                                  >?= tryU64 in // 2
     match underlyingAmount with
@@ -104,8 +104,8 @@ let getUnderlyingAmount dict =
     | None ->
         RT.failw "Message Body must include valid UnderlyingAmount"
 
-val getPairAsset: option (Dict.t data) -> result asset `cost` 198
-let getPairAsset dict =
+val getPairAsset: option (Dict.t data) -> result asset `cost` 241
+let getPairAsset dict = // 43
     let! version = dict >!= Dict.tryFind "PairAssetVersion" // 64
                         >?= tryU32 in // 2
     let! contractHash = dict >!= Dict.tryFind "PairContractHash" // 64
@@ -122,8 +122,8 @@ let getPairAsset dict =
     | _, _, None ->
         RT.failw "Message Body must include valid PairSubIdentifier"
 
-val getOrderTotal: option (Dict.t data) -> result U64.t `cost` 66
-let getOrderTotal dict =
+val getOrderTotal: option (Dict.t data) -> result U64.t `cost` 79
+let getOrderTotal dict = // 13
     let! orderTotal = dict >!= Dict.tryFind "OrderTotal" // 64
                            >?= tryU64 in // 2
     match orderTotal with
@@ -134,8 +134,8 @@ let getOrderTotal dict =
     | None ->
         RT.failw "Message Body must include valid OrderTotal"
 
-val getMakerPK: option (Dict.t data) -> result publicKey `cost` 66
-let getMakerPK dict =
+val getMakerPK: option (Dict.t data) -> result publicKey `cost` 77
+let getMakerPK dict = // 11
     let! makerPK = dict >!= Dict.tryFind "MakerPK" // 64
                         >?= tryPublicKey in // 2
     match makerPK with
@@ -144,8 +144,8 @@ let getMakerPK dict =
     | None ->
         RT.failw "Message Body must include valid MakerPK"
 
-val getReturnAddress: option (Dict.t data) -> result lock `cost` 66
-let getReturnAddress dict =
+val getReturnAddress: option (Dict.t data) -> result lock `cost` 77
+let getReturnAddress dict = // 11
     let! returnAddress = dict >!= Dict.tryFind "returnAddress" // 64
                               >?= tryLock in // 2
     match returnAddress with
@@ -154,13 +154,13 @@ let getReturnAddress dict =
     | None ->
         RT.failw "Message Body must include valid returnAddress"
 
-val getOrderAsset: contractId -> order -> asset `cost` 2328
-let getOrderAsset contractID order =
-    let! orderHash = hashOrder order in // 2328
-    mkAsset contractID orderHash
+val getOrderAsset: contractId -> order -> asset `cost` 2393
+let getOrderAsset contractID order = // 5
+    let! orderHash = hashOrder order in // 2384
+    mkAsset contractID orderHash // 4
 
-val getRequestedPayout: option (Dict.t data) -> result U64.t `cost` 66
-let getRequestedPayout dict =
+val getRequestedPayout: option (Dict.t data) -> result U64.t `cost` 79
+let getRequestedPayout dict = // 13
     let! requestedPayout = dict >!= Dict.tryFind "RequestedPayout" // 64
                                 >?= tryU64 in // 2
     match requestedPayout with
@@ -180,35 +180,35 @@ type makeParams = {
     makeOrderTotal: U64.t
 }
 
-val mkMakeParams: asset -> asset -> U64.t -> result makeParams `cost` 0
-let mkMakeParams underlyingAsset pairAsset orderTotal =
+val mkMakeParams: asset -> asset -> U64.t -> result makeParams `cost` 4
+let mkMakeParams underlyingAsset pairAsset orderTotal = // 4
     RT.ok ( { makeUnderlyingAsset=underlyingAsset;
               makePairAsset=pairAsset;
               makeOrderTotal=orderTotal } )
 
-val parseMake: option data -> result makeParams `cost` 466
-let parseMake messageBody =
+val parseMake: option data -> result makeParams `cost` 580
+let parseMake messageBody = // 11
     let! dict = messageBody >!= tryDict in // 4
-    let underlyingAsset = getUnderlyingAsset dict in // 198
-    let pairAsset = getPairAsset dict in // 198
-    let orderTotal = getOrderTotal dict in // 66
-    RT.bind3 underlyingAsset pairAsset orderTotal mkMakeParams
+    let underlyingAsset = getUnderlyingAsset dict in // 241
+    let pairAsset = getPairAsset dict in // 241
+    let orderTotal = getOrderTotal dict in // 79
+    RT.bind3 underlyingAsset pairAsset orderTotal mkMakeParams // 4
 
-val makeOrder: makeParams -> publicKey -> U64.t -> order `cost` 0
-let makeOrder makeParams senderPK underlyingAmount =
+val makeOrder: makeParams -> publicKey -> U64.t -> order `cost` 9
+let makeOrder makeParams senderPK underlyingAmount = // 9
     ret ( { underlyingAsset=makeParams.makeUnderlyingAsset;
             underlyingAmount=underlyingAmount;
             pairAsset=makeParams.makePairAsset;
             orderTotal=makeParams.makeOrderTotal;
             makerPubKey=senderPK } )
 
-val makeTx: txSkeleton -> contractId -> publicKey -> makeParams -> CR.t `cost` 2587
-let makeTx tx contractID senderPK makeParams =
+val makeTx: txSkeleton -> contractId -> publicKey -> makeParams -> CR.t `cost` 2696
+let makeTx tx contractID senderPK makeParams = // 35
     let! underlyingAmount = TX.getAvailableTokens makeParams.makeUnderlyingAsset tx in // 64
-    if underlyingAmount <> 0UL then begin // 2563
-        let! order = makeOrder makeParams senderPK underlyingAmount in
+    if underlyingAmount <> 0UL then begin // 2597
+        let! order = makeOrder makeParams senderPK underlyingAmount in // 9
         // issue a token with the hash of the order as the subidentifier, and lock it to the contract
-        let! orderAsset = getOrderAsset contractID order in // 2328
+        let! orderAsset = getOrderAsset contractID order in // 2393
         TX.mint 1UL orderAsset tx // 64
         >>= TX.lockToContract orderAsset 1UL contractID // 64
         // lock the underlying to the contract
@@ -217,12 +217,12 @@ let makeTx tx contractID senderPK makeParams =
         end
     else RT.autoFailw "UnderlyingAmount cannot be 0"
 
-val make: txSkeleton -> contractId -> sender -> option data -> CR.t `cost` 3053
-let make tx contractID sender messageBody =
+val make: txSkeleton -> contractId -> sender -> option data -> CR.t `cost` 3285
+let make tx contractID sender messageBody = // 9
     match sender with
     | PK senderPK ->
-        let makeParams = parseMake messageBody in // 466
-        makeParams `RT.bind` makeTx tx contractID senderPK // 2587
+        let makeParams = parseMake messageBody in // 580
+        makeParams `RT.bind` makeTx tx contractID senderPK // 2696
     | _ ->
         RT.autoFailw "Sender must authenticate with public key"
 
@@ -230,13 +230,13 @@ let make tx contractID sender messageBody =
 // Cancel an order
 //////////////////
 
-val getCancelOrder: publicKey -> option data -> result order `cost` 532
-let getCancelOrder makerPK messageBody =
+val getCancelOrder: publicKey -> option data -> result order `cost` 705
+let getCancelOrder makerPK messageBody = // 61
     let! dict = messageBody >!= tryDict in // 4
-    let! underlyingAsset = getUnderlyingAsset dict in // 198
-    let! underlyingAmount = getUnderlyingAmount dict in // 66
-    let! pairAsset = getPairAsset dict in // 198
-    let! orderTotal = getOrderTotal dict in // 66
+    let! underlyingAsset = getUnderlyingAsset dict in // 241
+    let! underlyingAmount = getUnderlyingAmount dict in // 79
+    let! pairAsset = getPairAsset dict in // 241
+    let! orderTotal = getOrderTotal dict in // 79
     match underlyingAsset, underlyingAmount, pairAsset, orderTotal with
     | OK underlyingAsset, OK underlyingAmount, OK pairAsset, OK orderTotal ->
         RT.ok ( { underlyingAsset=underlyingAsset;
@@ -256,10 +256,10 @@ val cancelTx:
     -> publicKey
     -> w: wallet
     -> order
-    -> CR.t `cost` (W.size w * 128 + 2587)
-let cancelTx tx contractID senderPK w order =
+    -> CR.t `cost` (W.size w * 128 + 2668)
+let cancelTx tx contractID senderPK w order = // 16
     // destroy the order
-    let! orderAsset = getOrderAsset contractID order in // 2328
+    let! orderAsset = getOrderAsset contractID order in // 2393
     begin TX.destroy 1UL orderAsset tx // 64
           >>= TX.fromWallet orderAsset 1UL contractID w // W.size w * 128 + 192
           <: option txSkeleton `cost` (W.size w * 128 + 256) end
@@ -271,14 +271,15 @@ val cancel:
     -> sender
     -> option data
     -> w: wallet
-    -> CR.t `cost` (W.size w * 128 + 3119)
-let cancel tx contractID sender messageBody w =
+    -> CR.t `cost` (W.size w * 128 + 3384)
+let cancel tx contractID sender messageBody w = // 11
     match sender with
     | PK senderPK ->
-        let order = getCancelOrder senderPK messageBody in // 532
-        order `RT.bind` cancelTx tx contractID senderPK w // W.size w * 128 + 2587
+        begin let order = getCancelOrder senderPK messageBody in // 705
+        order `RT.bind` cancelTx tx contractID senderPK w // W.size w * 128 + 2668
+        end <: CR.t `cost` (W.size w * 128 + 3373)
     | _ ->
-        RT.incFailw  (W.size w * 128 + 3119) "Sender must authenticate with public key"
+        RT.autoFailw "Sender must authenticate with public key"
 
 //////////////////
 // Taking an order
@@ -289,8 +290,8 @@ val checkRequestedPayout:
     order
     -> requestedPayout: U64.t
     -> paymentAmount: U64.t
-    -> bool `cost` 0
-let checkRequestedPayout { underlyingAmount=ua; orderTotal=ot} rp pa =
+    -> bool `cost` 153
+let checkRequestedPayout { underlyingAmount=ua; orderTotal=ot} rp pa = // 75
     // we want to check that
     // requestedPayout = floor (underlyingAmount * (paymentAmount / orderTotal))
     // which is equivalent to
@@ -303,9 +304,9 @@ let checkRequestedPayout { underlyingAmount=ua; orderTotal=ot} rp pa =
     let max64 = 18446744073709551615UL in
 
     // compute underlyingAmount * paymentAmount
-    let! ua_pa = dmul64 ua pa in
+    let! ua_pa = dmul64 ua pa in // 39
     // compute requestedPayout * orderTotal
-    let! rp_ot = dmul64 rp ot in
+    let! rp_ot = dmul64 rp ot in // 39
     // compute requestedPayout * orderTotal + orderTotal
     let rp_ot_ot = { hi = if rp_ot.lo >=^ max64 -%^ ot // will adding low 64 bits overflow
                           then rp_ot.hi +%^ 1UL // this never overflows
@@ -327,13 +328,13 @@ let checkRequestedPayout { underlyingAmount=ua; orderTotal=ot} rp pa =
     ret (ua_pa_lt_rp_ot_ot && rp_ot_ot_lte_ua_pa_ot)
 
 // parse the messageBody to get the order being taken
-val parseTake: option (Dict.t data) -> result order `cost` 594
-let parseTake dict =
-    let! underlyingAsset = getUnderlyingAsset dict in // 198
-    let! underlyingAmount = getUnderlyingAmount dict in // 66
-    let! pairAsset = getPairAsset dict in // 198
-    let! orderTotal = getOrderTotal dict in // 66
-    let! makerPK = getMakerPK dict in // 66
+val parseTake: option (Dict.t data) -> result order `cost` 794
+let parseTake dict = // 77
+    let! underlyingAsset = getUnderlyingAsset dict in // 241
+    let! underlyingAmount = getUnderlyingAmount dict in // 79
+    let! pairAsset = getPairAsset dict in // 241
+    let! orderTotal = getOrderTotal dict in // 79
+    let! makerPK = getMakerPK dict in // 77
     match underlyingAsset, underlyingAmount, pairAsset, orderTotal, makerPK with
     | OK underlyingAsset, OK underlyingAmount, OK pairAsset, OK orderTotal, OK makerPK ->
          RT.ok ({ underlyingAsset=underlyingAsset;
@@ -355,12 +356,12 @@ val updateOrder:
     -> U64.t
     -> U64.t
     -> txSkeleton
-    -> txSkeleton `cost` 2456
-let updateOrder contractID order paymentAmount payoutAmount tx = let open U64 in
+    -> txSkeleton `cost` 2547
+let updateOrder contractID order paymentAmount payoutAmount tx = let open U64 in // 26
     let newOrder = { order with
                      underlyingAmount=order.underlyingAmount-%^payoutAmount;
                      orderTotal=order.orderTotal-%^paymentAmount } in
-    let! newOrderAsset = getOrderAsset contractID newOrder in // 2328
+    let! newOrderAsset = getOrderAsset contractID newOrder in // 2393
     if paymentAmount <^ order.orderTotal // partial fill, so need to update the order
     then // mint new order asset and lock to contract
          TX.mint 1UL newOrderAsset tx // 64
@@ -375,22 +376,24 @@ val takeTx:
     -> U64.t
     -> order
     -> lock
-    -> CR.t `cost` (W.size w * 256 + 5767)
-let takeTx tx contractID wallet paymentAmount payoutAmount order returnAddress =
-    let! orderAsset = getOrderAsset contractID order in // 2328
-    let! makerPubKeyHash = hashPubkey order.makerPubKey in // 404
+    -> CR.t `cost` (W.size w * 256 + 5973)
+let takeTx tx contractID w paymentAmount payoutAmount order returnAddress = // 46
+    let! orderAsset = getOrderAsset contractID order in // 2393
+    let! makerPubKeyHash = hashPubkey order.makerPubKey in // 408
     // lock the underlying to the returnAddress
+    begin
     TX.lockToAddress order.underlyingAsset payoutAmount returnAddress tx // 64
     // lock the paymentAmount to the maker
     >>= TX.lockToPubKey order.pairAsset paymentAmount makerPubKeyHash // 64
     // destroy the order
     >>= TX.destroy 1UL orderAsset // 64
     //  create a new order if partial fill
-    >>= updateOrder contractID order paymentAmount payoutAmount // 2456
+    >>= updateOrder contractID order paymentAmount payoutAmount // 2547
     // add inputs from wallet
-    >>= TX.fromWallet order.underlyingAsset order.underlyingAmount contractID wallet // W.size wallet * 128 + 192
-    >?= TX.fromWallet orderAsset 1UL contractID wallet // W.size wallet * 128 + 192
+    >>= TX.fromWallet order.underlyingAsset order.underlyingAmount contractID w // W.size w * 128 + 192
+    >?= TX.fromWallet orderAsset 1UL contractID w // W.size w * 128 + 192
     >>= CR.ofOptionTxSkel "Could not find order in wallet. Ensure that both the order and the correct amount of the underlying are present." // 3
+    end <: CR.t `cost` (W.size w * 256 + 3126)
 
 val take':
     txSkeleton
@@ -399,26 +402,28 @@ val take':
     -> order
     -> U64.t
     -> lock
-    -> CR.t `cost` (W.size w * 256 + 5831)
-let take' tx contractID w order requestedPayout returnAddress =
+    -> CR.t `cost` (W.size w * 256 + 6210)
+let take' tx contractID w order requestedPayout returnAddress = // 20
+    begin
     let! paymentAmount = TX.getAvailableTokens order.pairAsset tx in // 64
-    let! paymentAmountOK = checkRequestedPayout order requestedPayout paymentAmount in // 0
+    let! paymentAmountOK = checkRequestedPayout order requestedPayout paymentAmount in // 153
     if paymentAmountOK
-    then takeTx tx contractID w paymentAmount requestedPayout order returnAddress // W.size w * 256 + 5767
-    else RT.incFailw (W.size w * 256 + 5767) "Incorrect requestedPayout"
+    then takeTx tx contractID w paymentAmount requestedPayout order returnAddress // W.size w * 256 + 5973
+    else RT.incFailw (W.size w * 256 + 5973) "Incorrect requestedPayout"
+    end <: CR.t `cost` (W.size w * 256 + 6190)
 
 val take:
     txSkeleton
     -> contractId
     -> option data
     -> w: wallet
-    -> CR.t `cost` (W.size w * 256 + 6561)
-let take tx contractID messageBody w =
+    -> CR.t `cost` (W.size w * 256 + 7178)
+let take tx contractID messageBody w = // 14
     let! dict = messageBody >!= tryDict in // 4
-    let order = parseTake dict in // 594
-    let requestedPayout = getRequestedPayout dict in // 66
-    let returnAddress = getReturnAddress dict in // 66
-    RT.bind3 order requestedPayout returnAddress (take' tx contractID w) // 5831
+    let order = parseTake dict in // 794
+    let requestedPayout = getRequestedPayout dict in // 79
+    let returnAddress = getReturnAddress dict in // 77
+    RT.bind3 order requestedPayout returnAddress (take' tx contractID w) // 6210
 
 //////////
 // exports
@@ -434,23 +439,23 @@ val main:
     -> w: wallet
     -> option data
     -> CR.t `cost` begin match command with
-                   | "Make" -> 3053
-                   | "Cancel" -> W.size w * 128 + 3119
-                   | "Take" -> W.size w * 256 + 6561
+                   | "Make" -> 3285
+                   | "Cancel" -> W.size w * 128 + 3384
+                   | "Take" -> W.size w * 256 + 7178
                    | _ -> 0 end
 let main tx _ contractID command sender messageBody w _ =
     match command with
     | "Make" ->
-        make tx contractID sender messageBody // 3053
+        make tx contractID sender messageBody // 3057
         <: CR.t `cost` begin match command with
-                       | "Make" -> 3053
-                       | "Cancel" -> W.size w * 128 + 3119
-                       | "Take" -> W.size w * 256 + 6561
+                       | "Make" -> 3285
+                       | "Cancel" -> W.size w * 128 + 3384
+                       | "Take" -> W.size w * 256 + 7178
                        | _ -> 0 end
     | "Cancel" ->
-        cancel tx contractID sender messageBody w // W.size w * 128 + 3119
+        cancel tx contractID sender messageBody w // W.size w * 128 + 3384
     | "Take" ->
-        take tx contractID messageBody w // W.size w * 256 + 6561
+        take tx contractID messageBody w // W.size w * 256 + 7178
     | _ ->
         RT.failw "Unrecognised command"
 
@@ -465,7 +470,7 @@ val cf:
     -> nat `cost` 0
 let cf _ _ command _ _ w _ =
     ret begin match command with
-        | "Make" -> 3053
-        | "Cancel" -> W.size w * 128 + 3119
-        | "Take" -> W.size w * 256 + 6561
+        | "Make" -> 3285
+        | "Cancel" -> W.size w * 128 + 3384
+        | "Take" -> W.size w * 256 + 7178
         | _ -> 0 end
