Dex001/README.md
@@ -1,5 +1,72 @@
 
-To verify/record hints, run `zebra  --z3rlimit 4500000 -v Dex001.fst`.  
+# ZenDex
+
+## Verify/Build
+
+To verify/record hints, run `zebra  --z3rlimit 7000000 -e Dex001.fst`.  
 This command may take a long time to run the first time.
 Subsequent runs will be significantly faster.
 With an AMD Threadripper 1950x @4.0GHz, recording hints takes ~67s. Subsequent runs take ~11s.
+
+## Usage
+
+ZenDex accepts three commands: `"Make"`, `"Cancel"`, and `"Take"`.
+
+### Making an order
+
+Use the command `"Make"`. You must sign with a public key -
+if the sender is `Anonymous` or `Contract contractID`, then the transaction will fail.
+
+The messageBody must consist of a dictionary which includes the following fields:
+
+| Field Name | Type | Description | Notes |
+|:----------:|:----:| ----------- | ----- |
+| `"UnderlyingAssetVersion"` | `UInt32` | The version number of the underlying asset | |
+| `"UnderlyingContractHash"` | `Hash`   | The contract hash for the underlying asset | |
+| `"UnderlyingSubIdentifier"`| `Hash`   | The asset sub-identifier for the underlying asset | |
+| `"PairAssetVersion"` | `UInt32` | The version number of the pair asset | |
+| `"PairContractHash"` | `Hash`   | The contract hash for the pair asset | |
+| `"PairSubIdentifier"` | `Hash`   | The asset sub-identifier for the pair asset | |
+| `"OrderTotal"` | `UInt64` | The total amount of the pair being ordered | Must be greater than 0 |
+
+The transaction must include a nonzero amount of the underlying asset being locked to ZenDex.
+
+For example, to make an order selling 50ZP for 1234 of some asset α which has asset identifier
+`00000000a0b1c2d3e4f5a6b7c8d9e0f1a2b3c4d5e6f7a8b9c0d1e2f3a4b5c6d7e8f9a0b1c2d3e4f5a6b7c8d9e0f1a2b3c4d5e6f7a8b9c0d1e2f3a4b5c6d7e8f9a0b1c2d3` -
+
+The messageBody would include the field-value pairs
+
+| Field Name | Type | Value | Notes |
+|:----------:|:----:| ----------- | ----- |
+| `"UnderlyingAssetVersion"` | `UInt32` | 0 | The ZP asset has version 0 |
+| `"UnderlyingContractHash"` | `Hash`   | `0000000000000000000000000000000000000000000000000000000000000000` | The ZP asset has the zero hash as it's contract hash |
+| `"UnderlyingContractHash"` | `Hash`   | `0000000000000000000000000000000000000000000000000000000000000000` | The ZP asset has the zero hash as it's asset sub-identifier |
+| `"PairAssetVersion"` | `UInt32` | `00000000` | The first 4 bytes of an asset identifier are the version number |
+| `"PairContractHash"` | `Hash`   | `a0b1c2d3e4f5a6b7c8d9e0f1a2b3c4d5e6f7a8b9c0d1e2f3a4b5c6d7e8f9a0b1` | The 5th to 36th bytes are the contract hash of the contract that generated the asset |
+| `"PairSubIdentifier"`| `Hash` | `c2d3e4f5a6b7c8d9e0f1a2b3c4d5e6f7a8b9c0d1e2f3a4b5c6d7e8f9a0b1c2d3` | The 37th to 68th bytes are the asset sub-identifier |
+| `"OrderTotal"` | `UInt64` | `1234` | The order is for 1234 of α |
+
+and the transaction would lock 50ZP to ZenDex.
+
+### Cancelling an order
+
+Use the command `"Cancel"`. You must sign with the public key that was used to create the order.
+
+The messageBody must consist of a dictionary which includes the following fields:
+
+| Field Name | Type | Description |
+|:----------:|:----:| ----------- |
+| `"UnderlyingAssetVersion"` | `UInt32` | The version number of the underlying asset of your order |
+| `"UnderlyingContractHash"` | `Hash`   | The contract hash for the underlying asset of your order |
+| `"UnderlyingSubIdentifier"`| `Hash`   | The asset sub-identifier for the underlying asset of your order |
+| `"UnderlyingAmount"` | `Hash` | The amount of the underlying in the order |
+| `"PairAssetVersion"` | `UInt32` | The version number of the pair asset of your order |
+| `"PairContractHash"` | `Hash` | The contract hash for the pair asset of your order |
+| `"PairSubIdentifier"` | `Hash` | The asset sub-identifier for the pair asset of your order |
+| `"OrderTotal"` | `UInt64` | The total amount of the pair ordered |
+
+the transaction must place the order asset in ZenDex's contract wallet.
+
+### Taking an order
+
+Use the command `"Take"`.
